First idea on stability

src/Language.v
@@ -14,7 +14,148 @@ From Coq Require Import List.
 Definition SomeZ (v: Z) := Some v.
 Coercion SomeZ: Z >-> option.
 
-Definition heap := Z -> option Z.
-Definition dom (h: heap): Ensemble Z :=
+Definition L := Z.
+
+Record heap: Set := mkheap {
+  hfun: L -> option Z;
+  hvar: list L;
+  hcond: forall x, In x hvar <-> hfun x <> None
+}.
+Coercion hfun: heap >-> Funclass.
+
+Definition dom (h: heap): Ensemble L :=
   fun n => h n <> None.
+
+Definition Partition (h h1 h2: heap): Prop :=
+  ((Included Z (dom h) (Union Z (dom h1) (dom h2)) /\
+    Disjoint Z (dom h1) (dom h2)) /\
+   (forall n, dom h1 n -> h n = h1 n)) /\
+  (forall n, dom h2 n -> h n = h2 n).
+
+Definition hfun_update (h: heap) (n: L) (v: Z): L -> option Z :=
+  fun m => if Z.eq_dec n m then v else h m.
+Definition hvar_update (h: heap) (n: L) (v: Z): list L :=
+  cons n (hvar h).
+Proposition hcond_update (h: heap) (n: L) (v: Z):
+    forall x, In x (hvar_update h n v) <-> (hfun_update h n v) x <> None.
+split; unfold hvar_update; unfold hfun_update; intro.
+- destruct H.
+  rewrite H; destruct (Z.eq_dec x x).
+  intro; inversion H0.
+  exfalso; apply n0; reflexivity.
+  unfold hfun_update.
+  destruct (Z.eq_dec n x).
+  intro; inversion H0.
+  apply hcond; assumption.
+- destruct (Z.eq_dec n x).
+  rewrite e; constructor; reflexivity.
+  right. apply hcond; assumption.
+Qed.
+Definition heap_update (h: heap) (n: L) (v: Z): heap :=
+  mkheap (hfun_update h n v) (hvar_update h n v) (hcond_update h n v).
+
+Definition V := nat.
+
+Definition store := V -> Z.
+
+Definition store_update (s: store) (x: V) (v: Z): store :=
+  fun y => if Nat.eq_dec x y then v else s y.
+
+Definition eq_restr (s t: store) (z: list V): Prop :=
+  forall (x: V), In x z -> s x = t x.
+
+(* Expressions are shallow, but finitely based *)
+Record expr: Set := mkexpr {
+  eval: store -> Z;
+  evar: list V;
+  econd: forall (s t: store), eq_restr s t evar -> eval s = eval t
+}.
+Coercion eval: expr >-> Funclass.
+
+Record guard: Set := mkguard {
+  gval: store -> bool;
+  gvar: list V;
+  gcond: forall (s t: store), eq_restr s t gvar -> gval s = gval t
+}.
+Coercion gval: guard >-> Funclass.
+
+Proposition const_guard_cond (v: bool) (s t : store):
+  eq_restr s t nil -> v = v.
+intros. reflexivity.
+Qed.
+Definition const_guard (v: bool): guard :=
+  mkguard (fun s => v) nil (const_guard_cond v).
+Coercion const_guard: bool >-> guard.
+
+Inductive assert :=
+| test: guard -> assert
+| hasval: expr -> expr -> assert
+| land: assert -> assert -> assert
+| limp: assert -> assert -> assert
+| lforall: V -> assert -> assert
+| sand: assert -> assert -> assert
+| simp: assert -> assert -> assert.
+Coercion test: guard >-> assert.
+
+Definition lnot (p: assert): assert := (limp p false).
+Definition lor (p q: assert): assert := lnot (land (lnot p) (lnot q)).
+Definition lexists (x: V) (p: assert): assert := lnot (lforall x (lnot p)).
+
+(* Classical *)
+
+Fixpoint satisfy (h: heap) (s: store) (p: assert): Prop :=
+  match p with
+  | test g => g s = true
+  | hasval e e' => dom h (e s) /\ h (e s) = e' s
+  | land p q => satisfy h s p /\ satisfy h s q
+  | limp p q => satisfy h s p -> satisfy h s q
+  | lforall x p => forall v, satisfy h (store_update s x v) p
+  | sand p q => exists h1 h2, Partition h h1 h2 /\
+      satisfy h1 s p /\ satisfy h2 s q
+  | simp p q => forall h'' h', Partition h'' h h' ->
+      satisfy h' s p -> satisfy h'' s q
+  end.
+
+(* Stable assertions *)
+Definition stable (p: assert) := forall h s, satisfy h s (lnot (lnot p)) -> satisfy h s p.
+
+Proposition stable_simp (p q: assert): stable p -> stable q -> stable (simp p q).
+intros.
+unfold stable; intros.
+simpl; intros.
+apply H0.
+simpl; intros.
+simpl in H1; apply H1; intro.
+apply H4.
+eapply H5. apply H2. assumption.
+Qed.
+
+Fixpoint satisfy_i (h: heap) (s: store) (p: assert): Prop :=
+  match p with
+  | test g => g s = true
+  | hasval e e' => dom h (e s) /\ h (e s) = e' s
+  | land p q => satisfy_i h s p /\ satisfy_i h s q
+  | limp p q => forall h'' h', Partition h'' h h' -> satisfy_i h' s p -> satisfy_i h' s q
+  | lforall x p => forall v, satisfy_i h (store_update s x v) p
+  | sand p q => exists h1 h2, Partition h h1 h2 /\
+      satisfy_i h1 s p /\ satisfy_i h2 s q
+  | simp p q => forall h'' h', Partition h'' h h' ->
+      satisfy_i h' s p -> satisfy_i h'' s q
+  end.
+
+
+
+
+
+
+
+
+
+
+
+
+
+
+
+
 
